progress

src/guarding/lib/full_lifetime_2.v
@@ -2,6 +2,7 @@ Require Import guarding.guard.
 Require Import guarding.own_and.
 Require Import guarding.tactics.
 Require Import guarding.lib.boxes.
+Require Import guarding.lib.lifetime_internals_ra.
 
 Require Import stdpp.base.
 From iris.algebra Require Export cmra updates.
@@ -15,634 +16,6 @@ From iris.proofmode Require Import ltac_tactics.
 From iris.proofmode Require Import tactics.
 From iris.proofmode Require Import coq_tactics.
 From iris.base_logic.lib Require Export invariants.
-
-(** Leaf Lifetime Logic. Based loosely on RustBelt's lifetime logic. *)
-
-(* begin hide *)
-
-Inductive LtRa :=
-  | LtOk : (option (gset nat * gset nat)) → gmultiset nat → gset nat → LtRa
-  | LtFail.
-  
-Instance lt_op : Op LtRa := λ a b , match a, b with
-  | LtOk (Some o) a1 d1, LtOk None a2 d2 =>
-      LtOk (Some o) (a1 ⊎ a2) (d1 ∪ d2)
-  | LtOk None a1 d1, LtOk (Some o) a2 d2 =>
-      LtOk (Some o) (a1 ⊎ a2) (d1 ∪ d2)
-  | LtOk None a1 d1, LtOk None a2 d2 =>
-      LtOk None (a1 ⊎ a2) (d1 ∪ d2)
-  | _, _ => LtFail
-end.
-
-Definition lt_inv (a: LtRa) := match a with
-  | LtOk (Some (sa, sd)) a d =>
-      sd = d ∧ sa ∩ sd = ∅
-      ∧ ∀ m , (m ∈ sa → multiplicity m a = 2) ∧ (m ∉ sa → multiplicity m a = 0)
-  | _ => False
-end.
-
-Instance lt_valid : Valid LtRa := λ a , ∃ b , lt_inv (a ⋅ b).
-
-Instance lt_equiv : Equiv LtRa := λ a b , a = b.
-
-Instance lt_pcore : PCore LtRa := λ a , match a with
-  | LtOk o1 a1 d1 => Some (LtOk None ∅ d1)
-  | LtFail => Some LtFail
-end.
-
-Lemma lt_assoc : Assoc (=) lt_op.
-Proof.
-  unfold Assoc. intros x y z. unfold lt_op.
-  destruct x as [[o|] a d|], y as [[o1|] a1 d1|], z as [[o2|] a2 d2|]; trivial; f_equiv; (try set_solver); rewrite gmultiset_disj_union_assoc; trivial.
-Qed.
-  
-Lemma lt_comm : Comm (=) lt_op.
-Proof.
-  unfold Comm. intros x y. unfold lt_op.
-  destruct x as [[o|] a d|], y as [[o1|] a1 d1|]; trivial; f_equiv; (try set_solver); rewrite gmultiset_disj_union_comm; trivial.
-Qed.
-
-Lemma LtOk_incl_3 a b d1 d2
-  (d_incl: d1 ⊆ d2)
-  : LtOk a b d1 ≼ LtOk a b d2.
-Proof.
-  exists (LtOk None ∅ d2). destruct a as [a|]; unfold "⋅", lt_op; f_equiv; try set_solver.
-Qed.
-  
-Lemma multiset_subseteq_of_LtOk_incl o0 a0 d0 o1 a1 d1 o2 a2 d2
-  (incl: LtOk o0 a0 d0 ≡ LtOk o1 a1 d1 ⋅ LtOk o2 a2 d2)
-  : d1 ⊆ d0.
-Proof.
-  unfold "⋅", lt_op in incl; destruct o1, o2; inversion incl; set_solver.
-Qed.
-
-Definition lt_ra_mixin : RAMixin LtRa.
-Proof. split.
-  - typeclasses eauto.
-  - intros a b cx abe. rewrite abe. intros t. exists cx. intuition.
-  - typeclasses eauto.
-  - unfold Assoc. intros. apply lt_assoc.
-  - unfold Comm. intros. apply lt_comm.
-  - intros x cx peq. unfold pcore, lt_pcore in peq. destruct x as [o|].
-    + inversion peq. subst cx. unfold "⋅", lt_op. destruct o; f_equiv; set_solver.
-    + inversion peq. subst cx. trivial.
-  - intros x cx peq. unfold pcore, lt_pcore in peq. destruct x.
-    + inversion peq. subst cx. trivial.
-    + inversion peq. subst cx. trivial.
-    
-  - intros x y cx xley peq.
-      destruct x as [o a d|], y as [o1 a1 d1|]; destruct xley as [[o2 a2 d2|] equ];
-      unfold pcore, lt_pcore; unfold pcore, lt_pcore in peq; inversion peq; subst cx.
-      + exists (LtOk None ∅ d1); intuition.  apply LtOk_incl_3.
-          eapply multiset_subseteq_of_LtOk_incl. apply equ.
-      + unfold "⋅", lt_op in equ. inversion equ. destruct o; discriminate.
-      + exists LtFail. intuition. exists LtFail. trivial.
-      + exists LtFail. intuition. exists LtFail. trivial.
-      + unfold "⋅", lt_op in equ. inversion equ.
-      + unfold "⋅", lt_op in equ. inversion equ.
-      + exists LtFail. intuition. exists LtFail. trivial.
-      + exists LtFail. intuition. exists LtFail. trivial.
-  - intros x y. unfold "✓", lt_valid. intros t. destruct t as [b t].
-      rewrite <- lt_assoc in t. exists (lt_op y b). apply t.
-Qed.
-
-Canonical Structure ltO
-  := discreteO LtRa.
-  
-Canonical Structure ltR := discreteR LtRa lt_ra_mixin.
-
-Global Instance lt_cmra_discrete : CmraDiscrete ltR.
-Proof. apply discrete_cmra_discrete. Qed.
-
-Global Instance lt_unit : Unit LtRa := LtOk None ∅ ∅.
-
-Definition lt_ucmra_mixin : UcmraMixin LtRa.
-split; trivial.
-  - exists (LtOk (Some (∅, ∅)) ∅ ∅). unfold lt_inv. simpl; set_solver.
-  - intro x. destruct x as [o a d|]; simpl; trivial.
-      destruct o; trivial.
-      + unfold ε, lt_unit, "⋅", lt_op. f_equiv; set_solver.
-      + unfold ε, lt_unit, "⋅", lt_op. f_equiv; set_solver.
-Qed.
-
-Canonical Structure ltUR := Ucmra LtRa lt_ucmra_mixin.
-
-Inductive BorState :=
-  | Borrow : gset nat → gset nat → BorState
-  | Unborrow : gset nat → gset nat → gset nat → BorState.
-
-Definition gmap_bor_state := gmap slice_name BorState.
-Definition gmap_props Σ := gmap slice_name (iProp Σ).
-
-(* end hide *)
-
-Class llft_logicGpreS Σ := { llft_logic_inG : inG Σ ltUR ; exclG : inG Σ (exclR unitO) }.
-Class llft_logicGS Σ := LlftLogicG {
-  llft_inG : llft_logicGpreS Σ;
-  llft_name: gname;
-}.
-Local Existing Instance llft_logic_inG.
-Local Existing Instance exclG.
-Local Existing Instance llft_inG.
-
-Definition llft_logicΣ : gFunctors := #[ GFunctor ltUR ; GFunctor (exclR unitO) ].
-
-Global Instance subG_lt_logicΣ Σ : subG llft_logicΣ Σ → llft_logicGpreS Σ.
-Proof.
-  solve_inG.
-Qed.
-
-Section LlftHelperResources.
-  Context {Σ: gFunctors}.
-  Context `{!llft_logicGpreS Σ}.
-  Context `{!invGS Σ}.
-  
-  (* begin hide *)
-
-  Definition lt_state (sa sd : gset nat) := LtOk (Some (sa, sd)) ∅ sd.
-  Definition LtState γlt (sa sd : gset nat) : iProp Σ := own γlt (lt_state sa sd).
-
-  Definition dead (k: nat) := LtOk None ∅ ({[ k ]}).
-  Definition Dead γlt (k: nat) : iProp Σ := own γlt (dead k).
-
-  Definition alive (k: nat) := LtOk None ({[+ k +]}) ∅.
-  Definition Alive γlt (k: nat) : iProp Σ := own γlt (alive k).
-  
-  Definition AuthBorState (γlt: gname) (mbs: gmap_bor_state) : iProp Σ :=
-      own γlt (LtOk (Some (∅, ∅)) ∅ {[0]}).
-  Definition OwnBorState (γlt: gname) (sn: slice_name) (bs: BorState) : iProp Σ :=
-      own γlt (LtOk (Some (∅, ∅)) ∅ {[1]}).
-  
-  Definition default_dead : nat := 0.
-  
-  (*Local Instance timeless_auth_bor_state γlt mbs : Timeless (AuthBorState γlt mbs).
-    Admitted.*)
-    
-  (*Local Instance timeless_own_bor_state γlt sn bs : Timeless (OwnBorState γlt sn bs).
-    Admitted.*)
-    
-  Local Lemma get_all_deads γlt sa sd :
-      LtState γlt sa sd ==∗ LtState γlt sa sd ∗ (∀ d , ⌜d ∈ sd⌝ -∗ Dead γlt d). Admitted.
-  
-  Local Lemma alloc_bor_state γlt sn mbs bs :
-      (mbs !! sn = None) →
-      AuthBorState γlt mbs
-      ⊢ |==> AuthBorState γlt (<[ sn := bs ]> mbs) ∗ OwnBorState γlt sn bs.
-      Admitted.
-      
-  Local Lemma alloc_bor_state2 γlt sn mbs sa sd al de de' :
-      (mbs !! sn = None) →
-      (de = de' ∨ (¬(de' ## sd) ∧ ¬(de ## sd) ∧ de ⊆ sa ∪ sd)) →
-      LtState γlt sa sd ∗ AuthBorState γlt mbs
-      ⊢ |==> LtState γlt sa sd ∗ AuthBorState γlt (<[ sn := Borrow al de' ]> mbs) ∗ OwnBorState γlt sn (Borrow al de).
-      Admitted.
-      
-  Local Lemma alloc_fake_bor_state_tok γlt sn (alive dead : gset nat) k :
-      (k ∈ alive) →
-      Dead γlt k ⊢ |==> OwnBorState γlt sn (Borrow alive dead).
-      Admitted.
-      
-  Local Lemma alloc_fake_bor_state_lts γlt sn (sa sd: gset nat) (alive dead : gset nat) :
-      ¬(alive ## sd) →
-      LtState γlt sa sd
-       ⊢ |==> LtState γlt sa sd ∗ OwnBorState γlt sn (Borrow alive dead).
-      Admitted.
-      
-  Local Lemma update_bor_state_borrow_fix_dead γlt sn al de de' k k' :
-      (k ∈ de) →
-      (k' ∈ de') →
-      Dead γlt k ∗ Dead γlt k' ∗ OwnBorState γlt sn (Borrow al de) ==∗ OwnBorState γlt sn (Borrow al de').
-      Admitted.
-      
-  Local Lemma update_bor_state_borrow_lts γlt sn mbs sa sd alive dead bs' :
-      (alive ## sd) →
-      LtState γlt sa sd ∗ AuthBorState γlt mbs ∗ OwnBorState γlt sn (Borrow alive dead)
-      ⊢ |==> LtState γlt sa sd ∗ AuthBorState γlt (<[ sn := bs' ]> mbs) ∗ OwnBorState γlt sn bs'.
-      Admitted.
-  
-  Local Lemma update_bor_state_borrow_tok γlt sn mbs alive dead bs' :
-      ([∗ set] k ∈ alive , Alive γlt k)
-          ∗ AuthBorState γlt mbs ∗ OwnBorState γlt sn (Borrow alive dead)
-      ⊢ |==> AuthBorState γlt (<[ sn := bs' ]> mbs) ∗ OwnBorState γlt sn bs'.
-      Admitted.
-      
-  (*Local Lemma update_bor_state_unborrow γlt sn mbs bl al de bs' :
-      AuthBorState γlt mbs ∗ OwnBorState γlt sn (Unborrow bl al de)
-      ⊢ |==> AuthBorState γlt (<[ sn := bs' ]> mbs) ∗ OwnBorState γlt sn bs'.
-      Admitted.*)
-  
-  Local Lemma delete_bor_state_borrow_lts γlt sn mbs sa sd alive dead :
-      (alive ## sd) →
-      LtState γlt sa sd ∗ AuthBorState γlt mbs ∗ OwnBorState γlt sn (Borrow alive dead)
-        ⊢ |==> 
-      LtState γlt sa sd ∗ AuthBorState γlt (delete sn mbs). Admitted.
-      
-  Local Lemma delete_bor_state_unborrow γlt sn mbs bl al de :
-      AuthBorState γlt mbs ∗ OwnBorState γlt sn (Unborrow bl al de)
-      ⊢ |==> AuthBorState γlt (delete sn mbs).
-      Admitted.
-      
-  (*Local Lemma agree_bor_state_borrow_tok γlt sn mbs (alive dead : gset nat) :
-      ([∗ set] k ∈ alive , Alive γlt k)
-          ∗ AuthBorState γlt mbs ∗ OwnBorState γlt sn (Borrow alive dead)
-      ⊢ |==> ⌜mbs !! sn = Some (Borrow alive dead)⌝.
-      Admitted.*)
-      
-  Local Lemma agree_bor_state_borrow_lts γlt sn mbs (sa sd al de : gset nat) :
-      (al ## sd) →
-      LtState γlt sa sd
-          ∗ AuthBorState γlt mbs ∗ OwnBorState γlt sn (Borrow al de)
-      ⊢ ∃ de' , ⌜mbs !! sn = Some (Borrow al de') ∧ (de = de' ∨ (¬(de' ## sd) ∧ ¬(de ## sd) ∧ de ⊆ (sa ∪ sd)))⌝.
-      Admitted.
-      
-  Local Lemma agree_bor_state_unborrow γlt sn mbs bl al de :
-      AuthBorState γlt mbs ∗ OwnBorState γlt sn (Unborrow bl al de)
-      ⊢ ⌜mbs !! sn = Some (Unborrow bl al de)⌝.
-      Admitted.
-      
-  Local Lemma distinct_bor_state_borrow_borrow_lts γlt sn1 sn2 al1 de1 al2 de2 alive dead :
-      (al1 ## dead) →
-      (al2 ## dead) →
-      LtState γlt alive dead
-        ∗ OwnBorState γlt sn1 (Borrow al1 de1)
-        ∗ OwnBorState γlt sn2 (Borrow al2 de2)
-      ⊢ ⌜sn1 ≠ sn2⌝.
-      Admitted.
-  
-  Local Lemma lt_alloc :
-    ⊢ |==> ∃ γ , LtState γ ∅ ∅.
-  Proof.
-    apply own_alloc. unfold "✓", cmra_valid, ltR, lt_valid.
-    exists (LtOk None ∅ ∅). simpl; set_solver.
-  Qed.
-
-  Local Lemma update_helper (a b : LtRa)
-    (cond: ∀ z : ltR, lt_inv (a ⋅ z) → lt_inv (b ⋅ z))
-    : a ~~> b.
-  Proof.
-    rewrite cmra_discrete_total_update.
-    intros y ay. destruct ay as [t ay]. rewrite <- lt_assoc in ay.
-    have co := cond _ ay. exists t. rewrite <- lt_assoc. apply co.
-  Qed.
-
-  Local Lemma update_helper2 (x y : LtRa)
-    (cond: ∀ o a d , lt_inv (x ⋅ LtOk o a d) → lt_inv (y ⋅ LtOk o a d))
-    : x ~~> y.
-  Proof.
-    apply update_helper. intros z. destruct z as [o a d|].
-    - apply cond.
-    - intros lti. unfold lt_inv in lti.
-      replace (x ⋅ LtFail) with LtFail in lti. { contradiction. }
-      destruct x as [o a d|]; trivial. destruct o; trivial.
-  Qed.
-
-  Local Lemma new_lt γlt k sa sd :
-    (k ∉ sa) → (k ∉ sd) →
-    LtState γlt sa sd ==∗ LtState γlt (sa ∪ {[ k ]}) sd ∗ Alive γlt k ∗ Alive γlt k.
-  Proof.
-    intros k_sa k_sd.
-    setoid_rewrite <- own_op. setoid_rewrite <- own_op.
-    iIntros "a". iApply own_update. 2: { iFrame "a". } apply update_helper2.
-
-    intros o a d lti. destruct o as [s|].
-    - contradiction. (*unfold "⋅", lt_op, lt_state, lt_inv in lti. contradiction.*)
-    - simpl in lti. destruct lti as [sd_d [no_int fm]].
-      simpl. split. { set_solver. }
-      split. { set_solver. }
-      intro m. split. {
-          intro m_in. have fmm := fm m. destruct fmm as [fmm1 fmm2].
-          rewrite elem_of_union in m_in. destruct m_in as [m_in|m_k].
-          + rewrite gmultiset_disj_union_left_id.
-            rewrite multiplicity_disj_union.
-            have fmm11 := fmm1 m_in.
-            rewrite gmultiset_disj_union_left_id in fmm11. rewrite fmm11.
-            rewrite multiplicity_disj_union.
-            rewrite multiplicity_singleton_ne. { trivial. }
-            intro mk. subst m. apply k_sa. apply m_in.
-          + rewrite gmultiset_disj_union_left_id.
-            rewrite multiplicity_disj_union.
-            rewrite multiplicity_disj_union.
-            rewrite elem_of_singleton in m_k. rewrite m_k.
-            rewrite multiplicity_singleton.
-            have fmk := fm k. destruct fmk as [_ fmk0].
-            rewrite gmultiset_disj_union_left_id in fmk0.
-            rewrite fmk0; trivial.
-          }
-          intros m_not_in. rewrite not_elem_of_union in m_not_in.
-          destruct m_not_in as [m_sa m_k].
-          rewrite gmultiset_disj_union_left_id.
-          rewrite multiplicity_disj_union.
-          rewrite multiplicity_disj_union.
-          have fmm := fm m. destruct fmm as [_ fmm0]. 
-          rewrite gmultiset_disj_union_left_id in fmm0. rewrite fmm0; trivial.
-          rewrite not_elem_of_singleton in m_k.
-          rewrite multiplicity_singleton_ne; trivial.
-  Qed.
-
-  Local Lemma double_incl_lt_inv a b z' :
-    (a ≼ z') → (b ≼ z') → (✓ z') → ∃ z, a ≼ z ∧ b ≼ z ∧ lt_inv z.
-  Proof.
-    intros az bz valz. destruct valz as [t valz]. exists (z' ⋅ t).
-    split.
-    { destruct az as [t1 az]. rewrite az. exists (t1 ⋅ t). rewrite <- lt_assoc. trivial. }
-    split.
-    { destruct bz as [t1 bz]. rewrite bz. exists (t1 ⋅ t). rewrite <- lt_assoc. trivial. }
-    trivial.
-  Qed.
-
-  Local Lemma lt_state_incl_lt_ok sa sd sa1 sd1 a d 
-    : (lt_state sa sd ≼ LtOk (Some (sa1, sd1)) a d) → sa = sa1 ∧ sd = sd1.
-  Proof.
-    intros lts. destruct lts as [t lts].
-    destruct t as [[o|] a1 d1|].
-    - unfold lt_state in lts. unfold "⋅", lt_op in lts. inversion lts.
-    - unfold lt_state in lts. unfold "⋅", lt_op in lts. inversion lts. split; trivial.
-    - unfold lt_state in lts. unfold "⋅", lt_op in lts. inversion lts.
-  Qed.
-
-  Local Lemma alive_incl_lt_ok k sa1 sd1 a d
-    : (alive k ≼ LtOk (Some (sa1, sd1)) a d) → lt_inv (LtOk (Some (sa1, sd1)) a d) → k ∈ sa1.
-  Proof.
-    intros lts lti. destruct lts as [t lts].
-    destruct t as [[o|] a1 d1|].
-    - unfold alive in lts. unfold "⋅", lt_op in lts. inversion lts.
-        unfold lt_inv in lti. destruct lti as [_ [_ fm]]. have fmk := fm k.
-        have h : Decision (k ∈ sa1) by solve_decision. destruct h as [h|n]; trivial.
-        exfalso.
-        destruct fmk as [_ fmk]. have fmk1 := fmk n. subst a.
-        rewrite multiplicity_disj_union in fmk1.
-        rewrite multiplicity_singleton in fmk1. lia.
-    - inversion lts.
-    - inversion lts.
-  Qed.
-
-  Local Lemma dead_incl_lt_ok k sa1 sd1 a d
-    : (dead k ≼ LtOk (Some (sa1, sd1)) a d) → lt_inv (LtOk (Some (sa1, sd1)) a d) → k ∈ sd1.
-  Proof.
-    intros lts lti. destruct lts as [t lts].
-    destruct t as [[o|] a1 d1|].
-    - unfold dead in lts. unfold "⋅", lt_op in lts. inversion lts.
-        unfold lt_inv in lti. destruct lti as [sde _]. subst d. set_solver.
-    - inversion lts.
-    - inversion lts.
-  Qed.
-
-  Local Lemma alive_dead_contradiction k sa sd a d
-    : (lt_inv (LtOk (Some (sa, sd)) a d)) → (k ∈ sa) → (k ∈ sd) → False.
-  Proof.
-    intros lts lti. destruct lts as [_ [no_int _]]. set_solver.
-  Qed.
-
-  Local Lemma lt_state_alive γlt k sa sd :
-    LtState γlt sa sd ∧ Alive γlt k ⊢ ⌜ k ∈ sa ⌝.
-  Proof.
-    iIntros "P". iDestruct (and_own_discrete_ucmra with "P") as (z') "[o [%incl1 %incl2]]".
-    iDestruct (own_valid with "o") as "%valz".
-    iPureIntro.
-    have di := double_incl_lt_inv _ _ _ incl1 incl2 valz.
-    destruct di as [z [inc1 [inc2 lti]]].
-    destruct z as [[[sa1 sd1]|] a d|]; try contradiction.
-    have j := lt_state_incl_lt_ok _ _ _ _ _ _ inc1. destruct j as [j1 j2]. subst sa.
-    apply (alive_incl_lt_ok _ _ _ _ _ inc2). apply lti.
-  Qed.
-
-  Local Lemma lt_state_dead γlt k sa sd :
-    LtState γlt sa sd ∧ Dead γlt k ⊢ ⌜ k ∈ sd ⌝.
-  Proof.
-    iIntros "P". iDestruct (and_own_discrete_ucmra with "P") as (z') "[o [%incl1 %incl2]]".
-    iDestruct (own_valid with "o") as "%valz".
-    iPureIntro.
-    have di := double_incl_lt_inv _ _ _ incl1 incl2 valz.
-    destruct di as [z [inc1 [inc2 lti]]].
-    destruct z as [[[sa1 sd1]|] a d|]; try contradiction.
-    have j := lt_state_incl_lt_ok _ _ _ _ _ _ inc1. destruct j as [j1 j2]. subst sd.
-    apply (dead_incl_lt_ok _ _ _ _ _ inc2). apply lti.
-  Qed.
-
-  Local Lemma lt_alive_dead_false γlt k :
-    Alive γlt k ∧ Dead γlt k ⊢ False.
-  Proof.
-    iIntros "P". iDestruct (and_own_discrete_ucmra with "P") as (z') "[o [%incl1 %incl2]]".
-    iDestruct (own_valid with "o") as "%valz".
-    iPureIntro.
-    have di := double_incl_lt_inv _ _ _ incl1 incl2 valz.
-    destruct di as [z [inc1 [inc2 lti]]].
-    destruct z as [[[sa1 sd1]|] a d|]; try contradiction.
-    have j1 := alive_incl_lt_ok _ _ _ _ _ inc1.
-    have j2 := dead_incl_lt_ok _ _ _ _ _ inc2.
-    eapply alive_dead_contradiction. { apply lti. } { apply j1. apply lti. } { apply j2. apply lti. }
-  Qed.
-
-  Local Lemma kill_lt γlt k sa sd :
-    LtState γlt sa sd ∗ Alive γlt k ∗ Alive γlt k ==∗
-        LtState γlt (sa ∖ {[ k ]}) (sd ∪ {[ k ]}) ∗ Dead γlt k.
-  Proof.
-    setoid_rewrite <- own_op. setoid_rewrite <- own_op.
-    iIntros "a". iApply own_update. 2: { iFrame "a". } apply update_helper2.
-
-    intros o a d lti. destruct o as [s|].
-    - contradiction.
-    - simpl in lti. destruct lti as [sd_d [no_int fm]].
-      simpl. split. { set_solver. }
-      split. { set_solver. }
-      intro m. split. {
-          intro m_in. have fmm := fm m. destruct fmm as [fmm1 fmm2].
-          rewrite gmultiset_disj_union_left_id.
-          rewrite gmultiset_disj_union_left_id.
-          rewrite gmultiset_disj_union_left_id in fmm1.
-          rewrite multiplicity_disj_union in fmm1.
-          rewrite multiplicity_disj_union in fmm1.
-          rewrite elem_of_difference in m_in. destruct m_in as [m_in mk].
-          rewrite elem_of_singleton in mk.
-          rewrite multiplicity_singleton_ne in fmm1; trivial.
-          apply fmm1. apply m_in.
-      }
-          intro m_in. have fmm := fm m. destruct fmm as [fmm1 fmm2].
-          rewrite gmultiset_disj_union_left_id.
-          rewrite gmultiset_disj_union_left_id.
-          rewrite gmultiset_disj_union_left_id in fmm2.
-          rewrite multiplicity_disj_union in fmm1.
-          rewrite multiplicity_disj_union in fmm1.
-          rewrite not_elem_of_difference in m_in.
-          have h : Decision (m ∈ sa) by solve_decision. destruct h as [h|n].
-          + destruct m_in as [m_not_in_sa|mk].
-            * exfalso. apply m_not_in_sa. apply h.
-            * rewrite multiplicity_disj_union in fmm1.
-              have fmm1i := fmm1 h.
-              rewrite elem_of_singleton in mk. subst m. rewrite multiplicity_singleton in fmm1i.
-                rewrite multiplicity_empty in fmm1i. lia.
-          + have fmm2i := fmm2 n.
-            rewrite multiplicity_disj_union in fmm2i.
-            rewrite multiplicity_disj_union in fmm2i. lia.
-  Qed.
-
-  Local Lemma bigSepS_alive_equiv_own γlt a
-    (ne_emp: a ≠ ∅)
-      : ([∗ set] k ∈ a, Alive γlt k) ⊣⊢ own γlt (LtOk None (list_to_set_disj (elements a)) ∅).
-  Proof.
-    induction a as [|x T ? IH] using set_ind_L. 
-    - contradiction.
-    - have h : Decision (T = ∅) by solve_decision. destruct h as [h|n]; trivial.
-      + subst T. rewrite big_sepS_union; last by set_solver.
-        rewrite big_sepS_empty. rewrite big_sepS_singleton. unfold Alive, alive.
-        rewrite union_empty_r. rewrite elements_singleton. unfold list_to_set_disj.
-        rewrite bi.sep_emp. rewrite gmultiset_disj_union_right_id. trivial.
-      + rewrite big_sepS_union; last by set_solver.
-        rewrite (IH n). rewrite big_sepS_singleton. unfold Alive, alive.
-          rewrite <- own_op.
-          f_equiv.
-          unfold "⋅", cmra_op, ltR, lt_op. f_equiv; last by set_solver.
-          rewrite elements_union_singleton; trivial.
-  Qed.
-
-  Local Lemma lt_ok_none_left o a1 d1 a2 d2
-      : LtOk None a1 d1 ⋅ LtOk o a2 d2 = LtOk o (a1 ⊎ a2) (d1 ∪ d2).
-  Proof.
-    destruct o as [o|]; trivial.
-  Qed.
-
-  Local Lemma mult_list_to_set_disj_not_in (a: gset nat) (x: nat)
-    (not_in: x ∉ a) : multiplicity x (list_to_set_disj (elements a)) = 0.
-  Proof.
-  induction a as [|y b ? IH] using set_ind_L. 
-  - trivial.
-  - rewrite elements_union_singleton; trivial. rewrite list_to_set_disj_cons.
-      rewrite multiplicity_disj_union. rewrite IH; last by set_solver.
-      assert (x ≠ y) by set_solver. rewrite multiplicity_singleton_ne; trivial.
-  Qed.
-
-  Local Lemma mult_list_to_set_disj_in (a: gset nat) (x: nat)
-    (is_in: x ∈ a) : multiplicity x (list_to_set_disj (elements a)) = 1.
-  Proof.
-  induction a as [|y b ? IH] using set_ind_L. 
-  - rewrite elem_of_empty in is_in. contradiction.
-  - rewrite elements_union_singleton; trivial. rewrite list_to_set_disj_cons.
-      rewrite multiplicity_disj_union.
-      rewrite elem_of_union in is_in. destruct is_in as [ix|ib].
-      + rewrite elem_of_singleton in ix. subst x. rewrite mult_list_to_set_disj_not_in; trivial.
-          rewrite multiplicity_singleton. trivial.
-      + rewrite (IH ib). rewrite multiplicity_singleton_ne; trivial. intro x_eq_y.
-          subst x. contradiction.
-  Qed.
-
-  Local Lemma multiplicity_le o1 a1 d1 o2 a2 d2 x
-    : LtOk o1 a1 d1 ≼ LtOk o2 a2 d2 → multiplicity x a1 ≤ multiplicity x a2.
-  Proof.
-    intro incl. destruct incl as [t incl]. destruct t as [o3 a3 d3|].
-    - assert (a2 = a1 ⊎ a3) as X.
-        + unfold "⋅", lt_op in incl. destruct o1; destruct o3.
-          * inversion incl. * inversion incl; trivial. * inversion incl; trivial.
-          * inversion incl; trivial.
-        + subst a2. rewrite multiplicity_disj_union. lia.
-    - unfold "⋅", lt_op in incl. destruct o1; inversion incl.
-  Qed.
-
-  Local Lemma own_and_alive γlt (a1 a2 : gset nat)
-    : own γlt (LtOk None (list_to_set_disj (elements a1)) ∅)
-      ∧ own γlt (LtOk None (list_to_set_disj (elements a2)) ∅)
-      ⊢ own γlt (LtOk None (list_to_set_disj (elements (a1 ∪ a2))) ∅).
-  Proof.
-    iIntros "x".
-    iDestruct (and_own_discrete_ucmra_specific with "x") as "y"; last by iFrame "y".
-    intros w valw incl1 incl2.
-    destruct w as [o a d|].
-    - exists (LtOk o (a ∖ (list_to_set_disj (elements (a1 ∪ a2)))) d).
-      rewrite lt_ok_none_left. f_equiv.
-      + rewrite gmultiset_eq. intros x.
-          rewrite multiplicity_disj_union.
-          rewrite multiplicity_difference.
-          enough ((multiplicity x a ≥ multiplicity x (list_to_set_disj (elements (a1 ∪ a2))))).
-          { lia. }
-          have t1 := multiplicity_le _ _ _ _ _ _ x incl1.
-          have t2 := multiplicity_le _ _ _ _ _ _ x incl2.
-          have h : Decision (x ∈ a1) by solve_decision. destruct h as [h1|n1]; trivial.
-            *  rewrite mult_list_to_set_disj_in in t1; trivial.
-              rewrite mult_list_to_set_disj_in; last by set_solver.
-              lia.
-          * have q : Decision (x ∈ a2) by solve_decision. destruct q as [h2|n2]; trivial.
-            -- rewrite mult_list_to_set_disj_in in t2; trivial.
-              rewrite mult_list_to_set_disj_in; last by set_solver.
-              lia.
-            -- rewrite mult_list_to_set_disj_not_in; last by set_solver.
-              lia.
-      + set_solver.
-    - unfold "✓", cmra_valid, ucmra_cmraR, ucmra_valid, ltUR, lt_valid in valw.
-      destruct valw as [b valw].
-      replace (LtFail ⋅ b) with LtFail in valw. { contradiction. }
-      destruct b; trivial.
-  Qed.
-
-  Local Lemma alive_and_bigSepS γlt (a1 a2 : gset nat)
-    : ([∗ set] k ∈ a1, Alive γlt k) ∧ ([∗ set] k ∈ a2, Alive γlt k)
-      ⊢ [∗ set] k ∈ a1 ∪ a2, Alive γlt k.
-  Proof.
-    have h: Decision (a1 = ∅) by solve_decision. destruct h as [h1|n1].
-    { subst a1. rewrite big_sepS_empty. rewrite bi.emp_and.
-        rewrite big_sepS_union; last by set_solver.
-        rewrite big_sepS_empty. rewrite bi.emp_sep. trivial. }
-    have h: Decision (a2 = ∅) by solve_decision. destruct h as [h2|n2].
-    { subst a2. rewrite big_sepS_empty. rewrite bi.and_emp.
-        rewrite big_sepS_union; last by set_solver.
-        rewrite big_sepS_empty. rewrite bi.sep_emp. trivial. }
-    rewrite bigSepS_alive_equiv_own; trivial.
-    rewrite bigSepS_alive_equiv_own; trivial.
-    rewrite bigSepS_alive_equiv_own; last by set_solver.
-    apply own_and_alive.
-  Qed.
-
-  Local Instance pers_dead γlt k : Persistent (Dead γlt k).
-  Proof.
-    apply own_core_persistent. unfold CoreId. trivial.
-  Qed.
-
-  Local Lemma LtState_entails_Dead γlt k sa sd : (k ∈ sd) → LtState γlt sa sd ⊢ Dead γlt k.
-  Proof.
-    intros ksd.
-    unfold LtState.
-    replace (lt_state sa sd) with (lt_state sa sd ⋅ dead k).
-    { rewrite own_op. iIntros "[A B]". iFrame "B". }
-    unfold dead, lt_state, "⋅", lt_op. f_equal. set_solver.
-  Qed.
-
-  Local Lemma LtState_disjoint γlt sa sd : LtState γlt sa sd ⊢ ⌜ sa ∩ sd = ∅ ⌝.
-  Proof.
-    iIntros "T". iDestruct (own_valid with "T") as "%val". iPureIntro.
-    destruct val as [t lts].
-    destruct t as [[o|] a d|].
-    - inversion lts.
-    - simpl in lts. intuition.
-    - inversion lts.
-  Qed.
-
-  Local Definition Cancel (γ: gname) : iProp Σ := own γ (Excl ()).
-  Local Lemma new_cancel : ⊢ |==> ∃ γ , Cancel γ.
-  Proof.
-    iIntros. iDestruct (own_alloc (Excl ())) as "H"; first done. unfold Cancel. iFrame "H".
-  Qed.
-  Local Lemma cancel_cancel_false (γc : gname) : Cancel γc ∗ Cancel γc ⊢ False.
-  Proof.
-    iIntros "X". unfold Cancel. rewrite <- own_op.
-    iDestruct (own_valid with "X") as "%J". contradiction.
-  Qed.
-
-  Local Lemma not_subset_eq_get (a b : gset nat) : (a ⊈ b) → ∃ k , k ∈ a ∧ k ∉ b.
-  Proof.
-    assert (∀ r , list_to_set r ⊈ b → ∃ u: nat , u ∈ ((list_to_set r) : gset nat) ∧ u ∉ b) as X.
-    { intro r. induction r as [|a0 r IHr].
-      - intros emp. rewrite list_to_set_nil in emp. set_solver.
-      - intros not_in. rewrite list_to_set_cons in not_in.
-        destruct (decide (a0 ∈ b)); trivial.
-        + assert (list_to_set r ⊈ b) as K by set_solver.
-          have IHr2 := IHr K. destruct IHr2 as [u IHr2]. exists u. set_solver.
-        + exists a0. intuition. rewrite list_to_set_cons. set_solver.
-    }
-    intro a_not_in_b.
-    have X1 := X (elements (Elements := gset_elements) a).
-    assert (list_to_set (elements a) ⊈ b) as Y. { set_solver. }
-    have Z := X1 Y. destruct Z as [u [Z1 Z2]]. exists u. split; trivial.
-    rewrite list_to_set_elements in Z1. trivial.
-  Qed.
-End LlftHelperResources.
 
 Section FullBorrows.
   (* (A, B) means A must end before B
@@ -1180,15 +553,84 @@ Section FullBorrows.
     }
   Qed. 
   
-  Lemma llft_fb_borrow_create_empty alive dead blocked lt P :
-      (lt ⊆ alive ∪ dead) →
+  Lemma llft_fb_vs_create_empty alive dead outlives mbs mprops sn P dd :
+  ¬(dd ## dead) →
+  (mbs !! sn = None) →
+  llft_fb_vs alive dead outlives mbs mprops
+  ⊢ llft_fb_vs alive dead outlives (<[sn:=Borrow ∅ dd]> mbs) (<[sn:=P]> mprops).
+  Proof.
+    generalize dead. clear dead.
+    induction alive as [my_alive IH] using set_ind_strong. 
+    iIntros (my_dead Hdd Hmbssn) "Hvs".
+    
+    rewrite llft_fb_vs_def.
+    rewrite (llft_fb_vs_def my_alive).
+    iIntros (k) "[[%Hin_my_alive %Hoc] [#Dead inval]]".
+    
+    iDestruct (full_borrows_invalidated_via_insert_false my_alive my_dead k sn mbs mprops (Borrow ∅ {[default_dead]}) P with "inval") as "inval"; trivial.
+    
+    iMod ("Hvs" $! k with "[inval]") as "[reval vs]". { iFrame. iFrame "Dead".
+      iPureIntro. intuition. }
+    
+    iModIntro.
+    
+    iSplitL "reval". {
+      iApply full_borrows_revalidated_via_insert_false; trivial.
+      unfold revalidated. rewrite bool_decide_eq_false. set_solver.
+    }
+    
+    iApply IH; trivial. { set_solver. }
+  Qed.
+  
+  Lemma llft_fb_borrow_create_empty alive dead blocked P :
       (▷ llft_fb_inv alive dead blocked) ∗ P
         ={↑Nbox}=∗
         ∃ sn , (▷ llft_fb_inv alive dead blocked)
             ∗ OwnBorState γ sn (Borrow ∅ {[ default_dead ]})
             ∗ slice Nbox sn P.
-  Admitted.
+  Proof.
+    iIntros "[Inv P]".
+    unfold llft_fb_inv.
+    iDestruct "Inv" as (mbs mprops Ptotal outlives) "[>auth [box [vs [>%pures [#slices outlives]]]]]".
     
+    iMod (slice_insert_full Nbox (↑Nbox) true (boxmap alive dead mbs) Ptotal P with "P box") as (sn) "[%Hisnone [#slice box]]"; trivial.
+    assert (mbs !! sn = None) as Hmbssn. {
+      destruct (mbs !! sn) eqn:Heqn; trivial.
+      rewrite lookup_fmap in Hisnone. rewrite Heqn in Hisnone. discriminate.
+    }
+    iMod (alloc_bor_state γ sn mbs (Borrow ∅ {[ default_dead ]}) with "auth") as "[auth OwnBor]"; trivial.
+    
+    assert (default_dead ∈ dead) as Hdd. { unfold map_wf in pures. intuition. }
+    assert (¬({[default_dead]} ## dead)) as Hdd2. { set_solver. }
+    
+    iDestruct (bi.later_mono _ _ (llft_fb_vs_create_empty alive dead outlives mbs mprops sn P {[default_dead]} Hdd2 Hmbssn) with "vs") as "vs".
+    
+    iModIntro. iExists sn. iFrame "OwnBor". iFrame "slice".
+    iNext.
+    iExists (<[sn:=Borrow ∅ {[default_dead]}]> mbs).
+    iExists (<[sn:=P]> mprops).
+    iExists (P ∗ Ptotal)%I.
+    iExists outlives.
+    iFrame "auth".
+    iSplitL "box". { 
+      rewrite boxmap_insert_Borrow.
+      rewrite bool_decide_eq_true_2. { iFrame. }
+      set_solver.
+    }
+    iFrame "vs". iFrame "outlives".
+    
+    destruct pures as [Hdom [Hwf Hoc]].
+    
+    iSplitL. { iPureIntro. 
+      split. { rewrite dom_insert_L. rewrite dom_insert_L. rewrite Hdom. trivial. }
+      split. { apply map_wf_insert; trivial. set_solver. }
+      trivial.
+    }
+    { iApply big_sepM_insert_1. iFrame "slice".
+      rewrite big_sepM_forall. iIntros (x R) "%Dm".
+      iApply "slices". iPureIntro. trivial. }
+  Qed.
+
   Lemma llft_fb_augment_outlives alive dead blocked outlives outlives' :
     (outlives ⊆ outlives') →
       (▷ llft_fb_inv alive dead blocked) ∗ Outlives outlives
